new/golang/defn/typing.v
@@ -1,225 +1,77 @@
-From Perennial.goose_lang Require Export lang notation.
+From stdpp Require Export pretty.
+From New.golang.defn Require Export intoval.
 From Perennial Require Import base.
 
-Definition go_string := byte_string.
-Delimit Scope byte_string_scope with go.
-Bind Scope byte_string_scope with go_string.
-(* NOTE: this causes W8 values to be printed using the byte notation set up in
-ByteString.v *)
-(* Delimit Scope byte_char_scope with go_byte. *)
+Module go.
+Definition identifier := go_string.
+Definition type_name := go_string.
 
-Inductive go_type :=
-(* Boolean *)
-| boolT
+(** https://go.dev/ref/spec#Types *)
+Inductive type :=
+| Named : type_name → type_args → _
+| TypeLit : type_lit → _
 
-(* Numeric, except float and impl-specific sized objects *)
-| uint8T
-| uint16T
-| uint32T
-| uint64T
-    (*
-| int8T
-| int16T
-| int32T
-| int64T *)
+with type_args := | TypeArgs : list type → _
 
-| stringT
-| arrayT (n : nat) (elem : go_type)
-| sliceT
-| interfaceT
-| structT (decls : list (go_string * go_type)) (* What if this were a gmap? *)
-| ptrT (* Untyped pointer; convenient to support recursion in structs *)
-| funcT
-.
+with type_lit :=
+| ArrayType : Z → type → _
+| StructType : list field_decl → _
+| PointerType : type → _
+| FunctionType : signature → _
+| InterfaceType : (list interface_elem) → _
+| SliceType : type → _
+| MapType : type → type → _
+| ChannelType : option bool → type → _
 
-Definition mapT (key elem : go_type) : go_type := ptrT.
-Definition chanT (elem : go_type) : go_type := ptrT.
+with field_decl :=
+| FieldDecl : (list go_string) → type → _
+| EmbeddedField : bool → go_string → type_args → _
 
-(* XXX: these are the same as the unsigned types because we want to have a 1-to-1 mapping
-   between Go types and the Coq types that represent them, and there's only a
-   single `w64` type representing both signed and unsigned integers.
- *)
-Definition int8T := uint8T.
-Definition int16T := uint16T.
-Definition int32T := uint32T.
-Definition int64T := uint64T.
+with signature := | Signature : parameters → result → _
 
-(* The zero_value for [floatX] is 0, so this is OK. *)
-Definition float32T := uint32T.
-Definition float64T := uint64T.
+with parameters := | ParameterList : (list parameter_decl) → _
 
-Class IntoVal `{ffi_syntax} (V : Type) :=
+with parameter_decl := | ParameterDecl : (list identifier) → (* variadic *) bool → _
+
+with result :=
+| ResultParameters : parameters → _
+| ResultType : type → _
+
+with interface_elem :=
+| MethodElem : identifier → signature → _
+| TypeElem : list type_term → _
+
+with type_term := | TypeTerm (type : type) | TypeTermUnderlying (type : type).
+
+Coercion TypeLit : type_lit >-> type.
+
+Definition string_to_go_string (s : string) : go_string :=
+  byte_to_w8 <$> String.list_byte_of_string s.
+
+Definition go_string_to_string (gs : go_string) : string :=
+  String.string_of_list_byte $ w8_to_byte <$> gs.
+
+Definition pretty_go `{!Pretty A} (a : A) : go_string :=
+  string_to_go_string (pretty a).
+
+(* Convert to string for comparison purposes and method lookups. *)
+Fixpoint type_to_string (t : type) : go_string :=
+  match t with
+  | Named n args => n
+  | ArrayType n elem => ("[" ++ pretty_go n ++ "]" ++ type_to_string elem)%go
+  | _ => ""%go
+  end.
+End go.
+
+(** FIXME: document this. Convenient for stating assumptions. Allows for
+    mutually recursive types in which e.g. the pointer element is not erased. *)
+Class NamedUnderlyingTypes :=
   {
-    to_val_def : V → val;
+    named_to_underlying : go_string -> (list go.type) → go.type
   }.
 
-Program Definition to_val := sealed @to_val_def.
-Definition to_val_unseal : to_val = _ := seal_eq _.
-Arguments to_val {_ _ _} v.
-(* Disable Notation "# l". *)
-Global Notation "# x" := (to_val x%go).
-Global Notation "#" := to_val.
-
-(* One of [V] or [ty] should not be an evar before doing typeclass search *)
-Global Hint Mode IntoVal - ! : typeclass_instances.
-
-Module func.
-Section defn.
-Context `{ffi_syntax}.
-Record t := mk {
-      f : binder;
-      x : binder;
-      e : expr;
-    }.
-Definition nil := mk <> <> (LitV LitPoison).
-End defn.
-End func.
-
-Section primitive_instances.
-Context `{ffi_syntax}.
-
-Global Instance into_val_loc : IntoVal loc :=
-  {| to_val_def := λ v, (LitV $ LitLoc v) |}.
-
-Global Instance into_val_w64 : IntoVal w64 :=
-  {| to_val_def := λ v, (LitV $ LitInt v) |}.
-
-Global Instance into_val_w32 : IntoVal w32 :=
-  {| to_val_def := λ v, (LitV $ LitInt32 v) |}.
-
-Global Instance into_val_w16 : IntoVal w16 :=
-  {| to_val_def := λ v, (LitV $ LitInt16 v) |}.
-
-Global Instance into_val_w8 : IntoVal w8 :=
-  {| to_val_def := λ v, (LitV $ LitByte v) |}.
-
-Global Instance into_val_unit : IntoVal () :=
-  {| to_val_def := λ _, (LitV $ LitUnit) |}.
-
-Global Instance into_val_bool : IntoVal bool :=
-  {| to_val_def := λ b, (LitV $ LitBool b) |}.
-
-Global Instance into_val_go_string : IntoVal go_string :=
-  {| to_val_def := λ s, (LitV $ LitString s) |}.
-
-Global Instance into_val_func : IntoVal func.t :=
-  {| to_val_def := λ (f : func.t), RecV f.(func.f) f.(func.x) f.(func.e) |}.
-End primitive_instances.
-
-Module slice.
-Record t := mk { ptr_f: loc; len_f: u64; cap_f: u64; }.
-Definition nil : slice.t := mk null 0 0.
-End slice.
-
-Module chan.
-  Definition t := loc.
-  Definition nil : chan.t := null.
-End chan.
-
-Module interface.
-Section goose_lang.
-  Context `{ffi_syntax}.
-
-  Inductive t :=
-  | mk (type_id : go_string) (v : val) : t
-  | nil : t.
-
-End goose_lang.
-End interface.
-
-Module struct.
-Definition descriptor := list (go_string * go_type).
-End struct.
-
-Section instances.
-Context `{ffi_syntax}.
-Global Instance into_val_array `{!IntoVal V} n : IntoVal (vec V n) :=
-  {| to_val_def :=
-      λ v, (Vector.fold_right PairV (vmap to_val v) #())
-  |}.
-
-Global Instance into_val_slice : IntoVal slice.t :=
-  {|
-    to_val_def (s: slice.t) := InjLV (#s.(slice.ptr_f), #s.(slice.len_f), #s.(slice.cap_f))
-  |}.
-
-Global Instance slice_eq_dec : EqDecision slice.t.
-Proof. solve_decision. Qed.
-
-Global Instance into_val_interface `{ffi_syntax} : IntoVal interface.t :=
-  {|
-    to_val_def (i: interface.t) :=
-      match i with
-      | interface.nil => NONEV
-      | interface.mk type_id v => SOMEV (#type_id, v)%V
-      end
-  |}.
-
-Global Instance into_val_prod `{!IntoVal A} `{!IntoVal B} : IntoVal (A * B) :=
-  {| to_val_def (v: A * B) := (PairV #(fst v) #(snd v)) |}.
-
-End instances.
-Global Notation "()" := tt : val_scope.
-
-Global Opaque to_val.
-
-Section val_types.
-
-  (* This type is never supposed to be used in real code; if you're ever forced
-     to deal with it in a proof, then something in Goose must have gone
-     wrong. *)
-  Definition badT_def := ptrT.
-  Program Definition badT := sealed @badT_def.
-  Definition badT_unseal : badT = _ := seal_eq _.
-
-  Definition byteT := uint8T.
-  Definition intT := int64T.
-  Definition uintT := uint64T.
-
-  Context `{ffi_syntax}.
-  Fixpoint zero_val_def (t : go_type) : val :=
-    match t with
-    | boolT => #false
-
-    (* Numeric, except float and impl-specific sized objects *)
-    | uint8T => #(W8 0)
-    | uint16T => #(W16 0)
-    | uint32T => #(W32 0)
-    | uint64T => #(W64 0)
-
-    | stringT => #""%V
-    | arrayT n elem => fold_right PairV #() (replicate n (zero_val_def elem))
-    | sliceT => #slice.nil
-    | structT decls => fold_right PairV #() (fmap (zero_val_def ∘ snd) decls)
-    | ptrT => #null
-    | funcT => #func.nil
-    | interfaceT => #interface.nil
-    end.
-  Program Definition zero_val := sealed @zero_val_def.
-  Definition zero_val_unseal : zero_val = _ := seal_eq _.
-
-  Fixpoint go_type_size_def (t : go_type) : nat :=
-    match t with
-    | structT d =>
-        (fix go_type_size_struct d : nat :=
-           match d with
-           | [] => O
-           | (_,t) :: d => (go_type_size_def t + go_type_size_struct d)%nat
-           end
-        ) d
-    | arrayT n e => n * (go_type_size_def e)
-    | _ => 1
-    end.
-  Program Definition go_type_size := sealed @go_type_size_def.
-  Definition go_type_size_unseal : go_type_size = _ := seal_eq _.
-End val_types.
-
-Reserved Notation "l +ₗ[ t ] z" (at level 50, left associativity, format "l  +ₗ[ t ]  z").
-Notation "l +ₗ[ t ] z" := (l +ₗ go_type_size t * z) : stdpp_scope .
-Notation "e1 +ₗ[ t ] e2" := (BinOp (OffsetOp (go_type_size t)) e1%E e2%E) : expr_scope .
-
-(* Shortcircuit Boolean connectives *)
-Notation "e1 && e2" :=
-  (If e1%E e2%E #false) (only parsing) : expr_scope.
-Notation "e1 || e2" :=
-  (If e1%E #true e2%E) (only parsing) : expr_scope.
+Definition to_underlying `{!NamedUnderlyingTypes} (t : go.type) : go.type :=
+  match t with
+  | go.Named n (go.TypeArgs args) => (named_to_underlying n args)
+  | _ => t
+  end.
