new/golang/defn/go_mem.v
@@ -1,0 +1,8 @@
+From New.golang.defn Require Export typing mem.
+From Perennial Require Import base.
+
+
+Reserved Notation "![ t ] e" (at level 9, right associativity, format "![ t ]  e").
+Notation "![ t ] e" := (mem.load t e%E) : expr_scope.
+Reserved Notation "e1 <-[ t ] e2" (at level 80, format "e1  <-[ t ]  e2").
+Notation "e1 <-[ t ] e2" := (mem.store t e1%E e2%E) : expr_scope.
