new/golang/defn/intoval.v
@@ -1,0 +1,120 @@
+From New.golang.defn Require Export notation.
+From Perennial Require Import base.
+
+Definition go_string := byte_string.
+Delimit Scope byte_string_scope with go.
+Bind Scope byte_string_scope with go_string.
+(* NOTE: this causes W8 values to be printed using the byte notation set up in
+ByteString.v *)
+(* Delimit Scope byte_char_scope with go_byte. *)
+
+Class IntoVal `{ffi_syntax} (V : Type) :=
+  {
+    to_val_def : V → val;
+  }.
+
+Program Definition to_val := sealed @to_val_def.
+Definition to_val_unseal : to_val = _ := seal_eq _.
+Arguments to_val {_ _ _} v.
+(* Disable Notation "# l". *)
+Global Notation "# x" := (to_val x%go).
+Global Notation "#" := to_val (at level 0).
+
+(* One of [V] or [ty] should not be an evar before doing typeclass search *)
+Global Hint Mode IntoVal - ! : typeclass_instances.
+
+Module func.
+Section defn.
+Context `{ffi_syntax}.
+Record t := mk {
+      f : binder;
+      x : binder;
+      e : expr;
+    }.
+Definition nil := mk <> <> (LitV LitPoison).
+End defn.
+End func.
+
+Section primitive_instances.
+Context `{ffi_syntax}.
+
+Global Instance into_val_loc : IntoVal loc :=
+  {| to_val_def := λ v, (LitV $ LitLoc v) |}.
+
+Global Instance into_val_w64 : IntoVal w64 :=
+  {| to_val_def := λ v, (LitV $ LitInt v) |}.
+
+Global Instance into_val_w32 : IntoVal w32 :=
+  {| to_val_def := λ v, (LitV $ LitInt32 v) |}.
+
+Global Instance into_val_w16 : IntoVal w16 :=
+  {| to_val_def := λ v, (LitV $ LitInt16 v) |}.
+
+Global Instance into_val_w8 : IntoVal w8 :=
+  {| to_val_def := λ v, (LitV $ LitByte v) |}.
+
+Global Instance into_val_unit : IntoVal () :=
+  {| to_val_def := λ _, (LitV $ LitUnit) |}.
+
+Global Instance into_val_bool : IntoVal bool :=
+  {| to_val_def := λ b, (LitV $ LitBool b) |}.
+
+Global Instance into_val_go_string : IntoVal go_string :=
+  {| to_val_def := λ s, (LitV $ LitString s) |}.
+
+Global Instance into_val_func : IntoVal func.t :=
+  {| to_val_def := λ (f : func.t), RecV f.(func.f) f.(func.x) f.(func.e) |}.
+End primitive_instances.
+
+Module slice.
+Record t := mk { ptr_f: loc; len_f: u64; cap_f: u64; }.
+Definition nil : slice.t := mk null 0 0.
+End slice.
+
+Module chan.
+  Definition t := loc.
+  Definition nil : chan.t := null.
+End chan.
+
+Module interface.
+Section goose_lang.
+  Context `{ffi_syntax}.
+
+  Inductive t :=
+  | mk (type_id : go_string) (v : val) : t
+  | nil : t.
+
+End goose_lang.
+End interface.
+
+Section instances.
+Context `{ffi_syntax}.
+Global Instance into_val_array `{!IntoVal V} n : IntoVal (vec V n) :=
+  {| to_val_def :=
+      λ v, (Vector.fold_right PairV (vmap to_val v) #())
+  |}.
+
+Global Instance into_val_slice : IntoVal slice.t :=
+  {|
+    to_val_def (s: slice.t) := InjLV (#s.(slice.ptr_f), #s.(slice.len_f), #s.(slice.cap_f))
+  |}.
+
+Global Instance slice_eq_dec : EqDecision slice.t.
+Proof. solve_decision. Qed.
+
+Global Instance into_val_interface `{ffi_syntax} : IntoVal interface.t :=
+  {|
+    to_val_def (i: interface.t) :=
+      match i with
+      | interface.nil => NONEV
+      | interface.mk type_id v => SOMEV (#type_id, v)%V
+      end
+  |}.
+
+Global Instance into_val_prod `{!IntoVal A} `{!IntoVal B} : IntoVal (A * B) :=
+  {| to_val_def (v: A * B) := (PairV #(fst v) #(snd v)) |}.
+
+End instances.
+Global Notation "()" := tt : val_scope.
+
+Global Opaque to_val.
